Atomic triples for BST verification

concurrency/verif_bst_conc_atomic.v
@@ -70,15 +70,6 @@ Arguments delete {V} x s.
 
 Eval hnf in reptype (nested_field_type t_struct_tree_t [StructField _lock]).
 
-Fixpoint tree_rep (t: tree val) (p: val) : mpred := (*tree strored in p correctly, see struct tree, representation in memory*)
- match t with
- | E => !!(p=nullval) && emp
- | T a x v b => !! (Int.min_signed <= x <= Int.max_signed /\ tc_val (tptr Tvoid) v) &&
-    EX pa:val, EX pb:val,
-    data_at Tsh t_struct_tree (Vint (Int.repr x),(v,(pa,pb))) p *
-    tree_rep a pa * tree_rep b pb
- end.
-
 
 Definition lsh1 := fst (slice.cleave Ews).
 Definition lsh2 := snd (slice.cleave Ews).
@@ -121,11 +112,14 @@ Qed.
 Hint Resolve readable_sh1 readable_sh2 sh1_sh2_join.
 
 Definition node_rep_r R arg : mpred := let '(np, t) := arg in
+ EX tp:val,
+ !!(is_pointer_or_null tp) &&
+(field_at Ews (t_struct_tree_t) [StructField _t] tp np) * malloc_token Ews t_struct_tree_t np * 
  match t with
- | E => !!(np=nullval) && emp
+ | E => !!(tp=nullval) && seplog.emp
  | T a x v b => !! (Int.min_signed <= x <= Int.max_signed /\ tc_val (tptr Tvoid) v) &&
-    EX pa : val, EX pb : val, EX locka : val, EX lockb : val, EX ga : gname, EX gb : gname,
-    data_at Ews t_struct_tree (Vint (Int.repr x),(v,(pa,pb))) np * malloc_token Ews t_struct_tree np *
+    EX tp:val, EX pa : val, EX pb : val, EX locka : val, EX lockb : val, EX ga : gname, EX gb : gname,
+    data_at Ews t_struct_tree (Vint (Int.repr x),(v,(pa,pb))) tp * malloc_token Ews t_struct_tree tp *
     lock_inv' locka ga a (uncurry R pa) * lock_inv' lockb gb b (uncurry R pb)
  end.
 
@@ -133,14 +127,20 @@ Definition node_rep_closed := HORec node_rep_r.
 
 Definition node_rep np t := node_rep_closed (np, t).
 
-Lemma node_rep_def : forall np t, node_rep np t =
- match t with
- | E => !!(np=nullval) && emp
+Definition tree_rep (tp:val) (t: tree val) :=
+match t with
+ | E => !!(tp=nullval) && seplog.emp
  | T a x v b => !! (Int.min_signed <= x <= Int.max_signed /\ tc_val (tptr Tvoid) v) &&
-    EX pa : val, EX pb : val, EX locka : val, EX lockb : val, EX ga : gname, EX gb : gname,
-    data_at Ews t_struct_tree (Vint (Int.repr x),(v,(pa,pb))) np * malloc_token Ews t_struct_tree np *
-    lock_inv' locka ga a (node_rep pa) * lock_inv' lockb gb b (node_rep pb)
- end.
+EX pa : val, EX pb : val, EX locka : val, EX lockb : val, EX ga : gname, EX gb : gname,
+    data_at Ews t_struct_tree (Vint (Int.repr x),(v,(pa,pb))) tp * malloc_token Ews t_struct_tree tp *
+    lock_inv' locka ga a (node_rep pa) * lock_inv' lockb gb b (node_rep pb) 
+   end.
+
+ Lemma node_rep_def : forall np t, node_rep np t =
+     EX tp:val,
+  !!(is_pointer_or_null tp) && 
+ (field_at Ews (t_struct_tree_t) [StructField _t] tp np) * malloc_token Ews t_struct_tree_t np *
+ tree_rep tp t.
 Proof.
   intros.
   unfold node_rep, node_rep_closed.
@@ -168,12 +168,12 @@ Proof.
   unfold t_lock_pred_r at 1.
   unfold t_lock_pred_closed.
   etransitivity; [|rewrite HORec_fold_unfold; auto]; reflexivity.
-Qed.*) Admitted.
+Qed.*) Admitted. 
 
-Definition ltree (t: tree val) lock p := EX g, lock_inv' lock g t (node_rep p).
+Definition ltree (t: tree val) (g:gname) lock p := lock_inv' lock g t (node_rep p).
 
-Definition nodebox_rep (sh : share) (lock : val) (nb: val) :=
- EX np: val, data_at sh (tptr (t_struct_tree_t)) np nb * field_at sh t_struct_tree_t [StructField _lock] lock np.
+Definition nodebox_rep (sh : share) (lock : val) (np: val ) (nb: val) :=
+data_at sh (tptr (t_struct_tree_t)) np nb * field_at sh t_struct_tree_t [StructField _lock] lock np.
 
 Definition surely_malloc_spec :=
   DECLARE _surely_malloc
@@ -188,64 +188,92 @@ Definition surely_malloc_spec :=
        PROP ()
        LOCAL (temp ret_temp p)
        SEP (mem_mgr gv; malloc_token Ews t p * data_at_ Ews t p).
-
-Definition treebox_new_spec :=
- DECLARE _treebox_new
-  WITH gv: globals
-  PRE  [  ]
-       PROP() LOCAL(gvars gv) SEP (mem_mgr gv)
-  POST [ tptr (tptr t_struct_tree_t) ]
-    EX v:val, EX lock:val,
-    PROP()
-    LOCAL(temp ret_temp v)
-    SEP (mem_mgr gv; nodebox_rep lsh1 lock v;
-           (* leftover slice of pointer *) data_at_ lsh2 (tptr t_struct_tree_t) v;
-           malloc_token Ews (tptr t_struct_tree_t) v).
-
-(*Definition insert_spec :=
- DECLARE _insert
-  WITH b: val, x: Z, v: val, t: tree val
-  PRE  [ _t OF (tptr (tptr t_struct_tree)), _x OF tint,
-        _value OF (tptr Tvoid)   ]
-    PROP( Int.min_signed <= x <= Int.max_signed; is_pointer_or_null v)
-    LOCAL(temp _t b; temp _x (Vint (Int.repr x)); temp _value v)
-    SEP (treebox_rep t b)
-  POST [ Tvoid ] 
-    PROP()
-    LOCAL()
-    SEP (treebox_rep (insert x v t) b).
-*)  
-    
-(*maybe I should add the treebox_rep in the ltree definition *)
-(*NEW*)
-Definition insert_spec :=
+       
+Program Definition insert_spec :=
   DECLARE _insert
-  WITH sh : share, lock : val,
-       b: val, x: Z, v: val, gv : globals
-  PRE [  _t OF (tptr (tptr t_struct_tree_t)), _x OF tint,
-        _value OF (tptr Tvoid)  ]
-   PROP (readable_share sh; Int.min_signed <= x <= Int.max_signed; is_pointer_or_null v)
-   LOCAL (temp _t b; temp _x (Vint (Int.repr x)); temp _value v; gvars gv)
-   SEP (mem_mgr gv; nodebox_rep sh lock b)
-  POST [ Tvoid ]
-   PROP ()
-   LOCAL ()
-   SEP (mem_mgr gv; nodebox_rep sh lock b).
-(*Definition insert_spec prog := DECLARE (ext_link_prog prog "insert") insert_spec'.*)    
+  ATOMIC TYPE (rmaps.ConstType ( val * val * share *  val * Z *val *globals * gname)) OBJ BST INVS empty top
+  WITH  b: _, np: _,  sh: _, lock : _,  x: _, v: _, gv : _ , g: _
+  PRE [  _t OF (tptr (tptr t_struct_tree_t)), _x OF tint,  _value OF (tptr tvoid)  ]
+          PROP (  readable_share sh; Int.min_signed <= x <= Int.max_signed;  is_pointer_or_null v; is_pointer_or_null lock)
+          LOCAL (temp _t b; temp _x (Vint (Int.repr x)); temp _value v; gvars gv)
+          SEPS  (mem_mgr gv * nodebox_rep sh lock np b) | ( ltree  BST g  lock np)   
+  POST[ tvoid  ]
+  EX b0: unit,
+        PROP ()
+        LOCAL ()
+       SEP (mem_mgr gv; nodebox_rep sh lock np b ; ltree   (insert x v BST) g lock np).
+   
 
-Definition lookup_spec :=
+Program Definition lookup_spec :=
  DECLARE _lookup
-  WITH sh : share, b: val, x: Z, lock : val
+   ATOMIC TYPE (rmaps.ConstType ( val * val *  Z * share * val  * gname)) OBJ BST INVS empty top
+  WITH  b: _, np : _,  x: _, sh:_, lock : _, g: _
   PRE  [ _t OF (tptr (tptr t_struct_tree_t(*t_struct_tree*))), _x OF tint  ]
     PROP(readable_share sh; Int.min_signed <= x <= Int.max_signed)
     LOCAL(temp _t b; temp _x (Vint (Int.repr x)))
-    SEP (nodebox_rep sh lock b)
+    SEPS (nodebox_rep sh lock np b) | ( ltree  BST g  lock np)   
   POST [ tptr Tvoid ]
    EX ret : val,
     PROP ()
     LOCAL(temp ret_temp ret)
-    SEP (nodebox_rep sh lock b).
-
+    SEP (!! (ret =  lookup(Vint (Int.repr x))  x  BST) && nodebox_rep sh lock np b;  ltree  BST g  lock np  ).
+    
+Program Definition treebox_free_spec :=
+ DECLARE _treebox_free
+   ATOMIC TYPE (rmaps.ConstType ( val* val * val * share * globals  * gname)) OBJ BST INVS empty top
+  WITH  lock: _, b:_,np:_, sh:_, gv: _, g:_
+  PRE  [ _b OF (tptr (tptr t_struct_tree_t)) ]
+       PROP(readable_share sh) 
+       LOCAL(gvars gv; temp _b b) 
+           SEPS (mem_mgr gv; nodebox_rep sh lock np b; malloc_token Ews (tptr t_struct_tree_t) b) | ( ltree  BST g  lock np)   
+  POST [ Tvoid ]
+  EX t : unit,
+    PROP()
+    LOCAL()
+    SEP (mem_mgr gv).
+    
+ Program Definition tree_free_spec :=
+ DECLARE _tree_free
+   ATOMIC TYPE (rmaps.ConstType ( val * val  * share * globals  * gname)) OBJ BST INVS empty top
+  WITH lock: _, np: _, sh:_, gv : _, g: _
+  PRE  [ _p OF (tptr t_struct_tree_t) ]
+       PROP(readable_share sh) 
+       LOCAL(gvars gv; temp _p np) 
+       SEPS (mem_mgr gv)|(ltree  BST g  lock np)
+  POST [ Tvoid ]
+    PROP()
+    LOCAL()
+    SEP (mem_mgr gv).
+ 
+ Program Definition delete_spec :=
+ DECLARE _delete
+    ATOMIC TYPE (rmaps.ConstType ( val * val * val * Z  * share   * gname)) OBJ BST INVS empty top
+      WITH lock: _, b: _, np: _, x: _, sh:_,  g: _
+  PRE  [ _t OF (tptr (tptr t_struct_tree)), _x OF tint]
+    PROP( readable_share sh ; Int.min_signed <= x <= Int.max_signed)
+    LOCAL(temp _t b; temp _x (Vint (Int.repr x)))
+    SEPS (nodebox_rep sh lock np b) | ( ltree  BST g  lock np)   
+  POST [ Tvoid ] 
+  EX t: unit,
+    PROP()
+    LOCAL()
+    SEP (nodebox_rep sh lock np b; ltree  (delete x  BST) g  lock np).
+    
+ Program Definition treebox_new_spec :=
+ DECLARE _treebox_new
+  WITH gv: globals, sh: share , g: gname
+   PRE  [ ]
+     PROP(readable_share sh)
+     LOCAL(gvars gv)
+     SEP (mem_mgr gv)
+  
+  POST [ tptr (tptr t_struct_tree_t) ]
+    EX b:val, EX np:val, EX lock:val,
+    PROP()
+    LOCAL(temp ret_temp b)
+    SEP (mem_mgr gv; nodebox_rep sh lock np b; ltree  E g  lock np;
+           malloc_token Ews (tptr t_struct_tree_t) b). 
+    
 Definition turn_left_spec :=
  DECLARE _turn_left
   WITH b: val, l: val, tl: val, x: Z, vx: val, tll: val, r: val, tr: val, y: Z, vy: val, mid: val, trr: val
@@ -268,7 +296,10 @@ Definition turn_left_spec :=
          data_at Ews t_struct_tree (Vint (Int.repr x), (vx, (tll, mid))) tl;
          data_at Ews t_struct_tree (Vint (Int.repr y), (vy, (l, trr))) tr).
 
-Definition pushdown_left_spec :=
+
+
+
+(* Definition pushdown_left_spec :=
  DECLARE _pushdown_left
   WITH b: val, p: val, tp: val, lockp: val, 
        x: Z, vx: val, locka: val, lockb: val, ta: val, tb: val,
@@ -303,25 +334,10 @@ Definition pushdown_left_spec :=
          ltree Ews ta locka;
          ltree Ews tb lockb *)
          (* nodebox_rep Ews locka ta;
-         nodebox_rep Ews lockb tb *)).
+         nodebox_rep Ews lockb tb *)). *)
 
-(* Definition pushdown_left_spec :=
- DECLARE _pushdown_left
-  WITH ta: tree val, x: Z, v: val, tb: tree val, b: val, p: val
-  PRE  [ _t OF (tptr (tptr (Tstruct _tree noattr)))]
-    PROP(Int.min_signed <= x <= Int.max_signed; tc_val (tptr Tvoid) v)
-    LOCAL(temp _t b)
-    SEP (data_at Tsh (tptr t_struct_tree) p b;
-         field_at Tsh t_struct_tree [StructField _key] (Vint (Int.repr x)) p;
-         field_at Tsh t_struct_tree [StructField _value] v p;
-         treebox_rep ta (field_address t_struct_tree [StructField _left] p);
-         treebox_rep tb (field_address t_struct_tree [StructField _right] p))
-  POST [ Tvoid ] 
-    PROP()
-    LOCAL()
-    SEP (treebox_rep (pushdown_left ta tb) b). *)
 
-Definition delete_spec :=
+(* Definition delete_spec :=
  DECLARE _delete
   WITH b: val, x: Z, t: tree val
   PRE  [ _t OF (tptr (tptr t_struct_tree)), _x OF tint]
@@ -332,7 +348,7 @@ Definition delete_spec :=
     PROP()
     LOCAL()
     SEP (treebox_rep (delete x t) b).
-
+ *)(* 
 Definition tree_free_spec :=
  DECLARE _tree_free
   WITH lock: val, p: val, gv : globals
@@ -399,7 +415,7 @@ Definition thread_func_spec :=
          PROP ()
          LOCAL ()
          SEP ().
-
+ *)
 Definition main_spec :=
  DECLARE _main
   WITH gv : globals
@@ -408,8 +424,8 @@ Definition main_spec :=
 
 
 Definition acquire_spec := DECLARE _acquire acquire_spec.
-Definition release2_spec := DECLARE _release2 release2_spec.
-Definition makelock_spec := DECLARE _makelock (makelock_spec _).
+Definition release2_spec := DECLARE _release2 release_spec.
+Definition makelock_spec := DECLARE _makelock (makelock_spec ).
 Definition freelock2_spec := DECLARE _freelock2 (freelock2_spec _).
 Definition spawn_spec := DECLARE _spawn spawn_spec.
 (*Definition freelock_spec := DECLARE _freelock (freelock_spec _).
@@ -424,39 +440,55 @@ Definition Gprog : funspecs :=
   (*
     acquire_spec; release_spec; makelock_spec; freelock_spec;
    makecond_spec; freecond_spec; wait_spec; signal_spec;*)
-    surely_malloc_spec; treebox_new_spec;
-    tree_free_spec; treebox_free_spec;
-    insert_spec; lookup_spec;
+    surely_malloc_spec;
+(*     tree_free_spec; treebox_free_spec; *)
+    insert_spec; (* lookup_spec;
     turn_left_spec; pushdown_left_spec; delete_spec ;
-    spawn_spec; thread_func_spec; main_spec 
+    spawn_spec; thread_func_spec;  *)main_spec 
   ]).
 
-Lemma node_rep_saturate_local:
-   forall t p, node_rep t p |-- !! is_pointer_or_null p.
-Proof.
+
+ Lemma node_rep_saturate_local:
+   forall t p, node_rep p t |-- !! is_pointer_or_null p.
+(* Proof.
 destruct t; simpl; intros.
-entailer!.
+entailer!. 
 Intros pa pb locka lockb. entailer!.
-Qed.
+Qed. *)
+Admitted.
 
 Hint Resolve node_rep_saturate_local: saturate_local.
 
-Lemma node_rep_valid_pointer:
-  forall t p, node_rep t p |-- valid_pointer p.
-Proof.
-intros.
-destruct t; simpl; normalize; auto with valid_pointer.
-Qed.
-Hint Resolve node_rep_valid_pointer: valid_pointer.
 
+Lemma node_rep_valid_pointer:
+  forall t p, node_rep p t |-- valid_pointer p.
+Proof.
+(*intros.
+destruct t; simpl; normalize; auto with valid_pointer.
+Qed. *)
+Admitted.
+
+
+Lemma tree_rep_valid_pointer:
+  forall t tp, tree_rep tp t |-- valid_pointer tp.
+Proof.
+(*intros.
+destruct t; simpl; normalize; auto with valid_pointer.
+Qed. *)
+Admitted.
+Hint Resolve tree_rep_valid_pointer : valid_pointer.
+
+(*
 Lemma ltree_saturate_local:
   forall lsh p lock, ltree lsh p lock |-- !! isptr p.
 Proof.
   intros; unfold ltree; entailer!.
 Qed.
-Hint Resolve ltree_saturate_local: saturate_local.
+Hint Resolve ltree_saturate_local: saturate_local. *)
 
-(*Lemma treebox_rep_saturate_local:
+(*
+ My comment 
+ Lemma treebox_rep_saturate_local:
    forall t b, treebox_rep t b |-- !! field_compatible (tptr t_struct_tree_t) [] b.
 Proof.
 intros.
@@ -466,22 +498,20 @@ entailer!.
 Qed.
 
 Hint Resolve treebox_rep_saturate_local: saturate_local.
-
-Definition insert_inv (b0: val) (t0: tree val) (x: Z) (v: val): environ -> mpred :=
-  EX b: val, EX t: tree val,
-  PROP()
-  LOCAL(temp _t b; temp _x (Vint (Int.repr x));   temp _value v)
-  SEP(treebox_rep t b;  (treebox_rep (insert x v t) b -* treebox_rep (insert x v t0) b0)). (* b0 which points to t0 which is the entire tree *)
 *)
+Notation ghost_ref_tree t g := ( ghost_reference (P:=discrete_PCM _) t g ).
 
-Definition insert_inv (b0: val) (lsh0 : share) (lock0 : val) (x: Z) (v: val) gv: environ -> mpred :=
-  EX p: val, EX lock: val,
+Definition insert_inv (b0: val) (tp0:val)  (lsh0 : share) (lock0 : val) (x: Z) (v: val) gv (t: tree val) (inv_names : invG) (Q : () -> mpred) ( g:gname) : environ -> mpred :=
   PROP()
-  LOCAL(temp _l lock; temp _tgt p; temp _x (Vint (Int.repr x)); temp _value v; gvars gv)
-  SEP(mem_mgr gv; |>lock_inv lsh2 lock (t_lock_pred p lock); t_lock_pred_base p lock;
-      nodebox_rep lsh0 lock0 b0).
+  LOCAL(temp _l lock0; temp _tgt tp0; temp _x (Vint (Int.repr x)); temp _value v; gvars gv)
+  SEP(mem_mgr gv;   nodebox_rep lsh0 lock0 tp0 b0; 
+  atomic_shift (λ a : tree val, lock_inv' lock0 g a (node_rep tp0)) ∅ ⊤
+  (λ (t : tree val) (_ : ()),
+     mem_mgr gv *
+     (nodebox_rep lsh0 lock0 tp0 b0 * (ltree (insert x v t) g lock0 tp0 * seplog.emp))) Q *
+ghost_ref_tree t g * node_rep tp0 t).
 
-
+(*
 Lemma ramify_PPQQ {A: Type} {NA: NatDed A} {SA: SepLog A} {CA: ClassicalSep A}: forall P Q,
   P |-- P * (Q -* Q).
 Proof.
@@ -500,7 +530,7 @@ Proof.
   Intros pa pb locka lockb. entailer!.
 Qed.
 
-Hint Resolve node_rep_nullval: saturate_local.
+Hint Resolve node_rep_nullval: saturate_local. *)
 
 (*Lemma treebox_rep_leaf: forall x p b (v: val),
   is_pointer_or_null v ->
@@ -572,6 +602,169 @@ Proof.
   cancel.
 Qed.
 *)
+
+Lemma body_insert: semax_body Vprog Gprog f_insert insert_spec.
+Proof.
+  start_function.
+  Intros. 
+  simpl.
+  unfold nodebox_rep at 2.
+  Intros.
+  forward.
+  forward.
+  forward_call  [tree val : Type; unit : Type] acquire_inv(lock,g, (node_rep np),
+    (λ (t : tree val) (_ : ()), mem_mgr gv *
+               ( nodebox_rep sh lock np b *
+               (ltree (insert x v t) g lock np * seplog.emp))), Q , inv_names ).
+               {   unfold ltree at 1. cancel. }
+  Intros BST.
+   eapply semax_pre; [
+    | apply (semax_loop _ (insert_inv b np sh lock x v gv BST inv_names Q g) (insert_inv b np sh lock  x v gv BST inv_names Q g) )]. 
+  * (* Precondition *)
+    unfold insert_inv.
+    unfold nodebox_rep at 2.
+    Intros.
+     entailer!. 
+  * (* Loop body *)
+    unfold insert_inv.
+    Intros.
+    forward. (* Sskip *)
+    rewrite node_rep_def. 
+    Intros tp.
+    forward. (*p=tgt->t*)
+    forward_if.
+    + (* then clause *)
+      subst tp.
+      forward_call (t_struct_tree_t, gv).
+      { simpl. repeat (split; auto); rep_omega. }
+      Intros p1'.
+      forward_call (t_struct_tree_t, gv).
+      { simpl. repeat (split; auto); rep_omega. }
+      Intros p2'.
+      forward. (* p1->t=NULL *)
+      simpl.
+      forward. (* p1->t=NULL *)
+      simpl. 
+      forward_call (tlock, gv).
+      { simpl. rewrite Z.max_r. repeat (split; auto); rep_omega. rep_omega. }
+      Intros l1.
+      unfold tlock.
+      forward_call [tree val : Type] makelock_inv (l1, BST, node_rep np).   
+      Intro g0.
+      Intros.    
+      forward. (*p1->lock = l1*) 
+(*       rewrite <- (lock_inv_share_join lsh1 lsh2) by auto. *)
+      forward_call [tree val : Type; tree val : Type] release_inv (l1, g, BST, node_rep np, fun (n n' : tree val) => emp,
+    (fun (_ : tree val) => emp), inv_names).
+Admitted.
+  (*     {  lock_props. 
+        rewrite t_lock_pred_def at 3. Exists (E : tree val) (vint 0).
+        unfold_data_at 2%nat. erewrite <- (field_at_share_join _ _ _ _ [StructField _lock]) by eauto.
+         simpl. entailer!. }
+      deadvars.
+      forward_call (tlock, gv).
+      { simpl. repeat (split; auto); rep_omega. }
+      Intros l2.
+      forward_call(l2, Ews, t_lock_pred p2' l2). 
+      forward. (*p2->lock = l2*)
+      rewrite <- (lock_inv_share_join lsh1 lsh2) by auto.
+      forward_call(l2, lsh2, t_lock_pred_base p2' l2, t_lock_pred p2' l2).
+      { lock_props.
+        rewrite t_lock_pred_def at 3. Exists (E : tree val) (vint 0).
+        unfold_data_at 1%nat. erewrite <- (field_at_share_join _ _ _ _ [StructField _lock]) by eauto.
+        simpl. entailer!. }
+      forward_call (t_struct_tree, gv).
+      { simpl. repeat (split; auto); rep_omega. }
+      Intros p'.
+      forward. (* tgt->t=p; *)  
+      forward. (* p->key=x; *)
+      forward. (* p->value=value; *)
+      forward. (* p->left=NULL; *)
+      forward. (* p->right=NULL; *)
+      assert_PROP (t1= (@E _)) by entailer!.
+      subst t1. simpl node_rep.
+      assert_PROP (field_compatible t_struct_tree_t [] p1) by entailer!.
+      forward_call(lock1, lsh2, t_lock_pred_base p1 lock1, t_lock_pred p1 lock1).
+      { lock_props.
+        setoid_rewrite t_lock_pred_def at 4.
+        Exists (T E x v E) p'. cancel. simpl. Exists p1' p2' l1 l2. unfold ltree. entailer!.
+        rewrite <- later_sepcon; eapply derives_trans; [|apply sepcon_derives, derives_refl; apply now_later].
+        entailer!.
+        { rewrite field_compatible_cons in H6, H8; destruct H6, H8; auto. } }
+      forward. (* return; *)
+    + (* else clause *)
+      destruct t1.
+      { simpl node_rep. normalize. }
+      simpl node_rep.
+      Intros pa pb locka lockb.
+      forward. (* y=p->key; *)
+      forward_if; [ | forward_if ].
+      - (* Inner if, then clause: x<k *)
+        forward.
+        forward.
+        unfold_data_at (data_at _ _ _ tp).
+        rewrite (field_at_data_at _ _ [StructField _left]); simpl.
+        assert_PROP (field_compatible t_struct_tree [StructField _left] tp) by entailer!.
+        rewrite field_compatible_field_address by auto.
+        unfold ltree at 1; Intros.
+        forward.
+        forward_call (locka, lsh1, t_lock_pred pa locka).
+        rewrite t_lock_pred_def at 2.
+        Intros ta tpa.
+        forward_call(lock1, lsh2, t_lock_pred_base p1 lock1, t_lock_pred p1 lock1).
+        { lock_props.
+          setoid_rewrite t_lock_pred_def at 4. Exists (T t1_1 k v0 t1_2) tp.
+          cancel. simpl. Exists pa pb locka lockb.
+          unfold ltree; entailer!.
+          unfold_data_at (data_at _ _ _ tp); cancel.
+          rewrite (field_at_data_at _ _ [StructField _left]), field_compatible_field_address by auto; simpl; cancel.
+          rewrite <- later_sepcon; eapply derives_trans; [|apply sepcon_derives, derives_refl; apply now_later].
+          cancel. }
+        Exists pa locka.
+        unfold ltree; entailer!.
+        unfold t_lock_pred_base.
+        Exists ta tpa; cancel.
+      - (* Inner if, second branch:  k<x *)
+        forward.
+        forward.
+        unfold_data_at (data_at _ _ _ tp).
+        rewrite (field_at_data_at _ _ [StructField _left]); simpl.
+        assert_PROP (field_compatible t_struct_tree [StructField _left] tp) by entailer!.
+        rewrite field_compatible_field_address by auto.
+        unfold ltree at 2; Intros.
+        forward.
+        forward_call (lockb, lsh1, t_lock_pred pb lockb).
+        rewrite t_lock_pred_def at 2.
+        Intros tb tpb.
+        forward_call(lock1, lsh2, t_lock_pred_base p1 lock1, t_lock_pred p1 lock1).
+        { lock_props.
+          setoid_rewrite t_lock_pred_def at 4. Exists (T t1_1 k v0 t1_2) tp.
+          cancel. simpl. Exists pa pb locka lockb.
+          unfold ltree; entailer!.
+          unfold_data_at (data_at _ _ _ tp); cancel.
+          rewrite (field_at_data_at _ _ [StructField _left]), field_compatible_field_address by auto; simpl; cancel.
+          rewrite <- later_sepcon; eapply derives_trans; [|apply sepcon_derives, derives_refl; apply now_later].
+          cancel. }
+        Exists pb lockb.
+        unfold ltree; entailer!.
+        unfold t_lock_pred_base.
+        Exists tb tpb; cancel.
+      - (* x = k *)
+        forward.
+        forward_call(lock1, lsh2, t_lock_pred_base p1 lock1, t_lock_pred p1 lock1).
+        { lock_props.
+          setoid_rewrite t_lock_pred_def at 2. Exists (T t1_1 k v t1_2) tp.
+          cancel. simpl. Exists pa pb locka lockb.
+          unfold ltree; entailer!.
+          rewrite <- later_sepcon; eapply derives_trans; [|apply sepcon_derives, derives_refl; apply now_later].
+          cancel. }
+        forward.
+  * (* After the loop *)
+    forward.
+    unfold loop2_ret_assert. apply andp_left2. normalize.
+Qed. *)
+
+
 Lemma modus_ponens_wand' {A}{ND: NatDed A}{SL: SepLog A}:
   forall P Q R: A, P |-- Q -> P * (Q -* R) |-- R.
 Proof.
@@ -1125,154 +1318,5 @@ Proof.
   forward. Exists p; entailer!.
 Qed.
 
-Lemma body_insert: semax_body Vprog Gprog f_insert insert_spec.
-Proof.
-  start_function.
-  unfold nodebox_rep; Intros p.
-  forward.
-  unfold ltree; Intros.
-  forward.
-  forward_call (lock, sh, t_lock_pred p lock).
-  eapply semax_pre; [
-    | apply (semax_loop _ (insert_inv b sh lock x v gv) (insert_inv b sh lock  x v gv) )].
-  * (* Precondition *)
-    unfold insert_inv.
-    rewrite t_lock_pred_def at 2; Intros t0 tp.
-    Exists p lock.
-    unfold ltree; entailer!.
-    unfold nodebox_rep, t_lock_pred_base.
-    Exists p t0 tp; unfold ltree; entailer!.
-  * (* Loop body *)
-    unfold insert_inv.
-    Intros p1 lock1.
-    forward. (* Sskip *)
-    unfold t_lock_pred_base; Intros t1 tp.
-    forward. (*p=tgt->t*)
-    forward_if.
-    + (* then clause *)
-      subst tp.
-      forward_call (t_struct_tree_t, gv).
-      { simpl. repeat (split; auto); rep_omega. }
-      Intros p1'.
-      forward_call (t_struct_tree_t, gv).
-      { simpl. repeat (split; auto); rep_omega. }
-      Intros p2'.
-      forward. (* p1->t=NULL *)
-      simpl.
-      forward. (* p1->t=NULL *)
-      simpl. 
-      forward_call (tlock, gv).
-      { simpl. repeat (split; auto); rep_omega. }
-      Intros l1.
-      forward_call(l1, Ews, t_lock_pred p1' l1). 
-      forward. (*p1->lock = l1*) 
-      rewrite <- (lock_inv_share_join lsh1 lsh2) by auto.
-      forward_call(l1, lsh2, t_lock_pred_base p1' l1, t_lock_pred p1' l1).
-      { lock_props.
-        rewrite t_lock_pred_def at 3. Exists (E : tree val) (vint 0).
-        unfold_data_at 2%nat. erewrite <- (field_at_share_join _ _ _ _ [StructField _lock]) by eauto.
-         simpl. entailer!. }
-      deadvars.
-      forward_call (tlock, gv).
-      { simpl. repeat (split; auto); rep_omega. }
-      Intros l2.
-      forward_call(l2, Ews, t_lock_pred p2' l2). 
-      forward. (*p2->lock = l2*)
-      rewrite <- (lock_inv_share_join lsh1 lsh2) by auto.
-      forward_call(l2, lsh2, t_lock_pred_base p2' l2, t_lock_pred p2' l2).
-      { lock_props.
-        rewrite t_lock_pred_def at 3. Exists (E : tree val) (vint 0).
-        unfold_data_at 1%nat. erewrite <- (field_at_share_join _ _ _ _ [StructField _lock]) by eauto.
-        simpl. entailer!. }
-      forward_call (t_struct_tree, gv).
-      { simpl. repeat (split; auto); rep_omega. }
-      Intros p'.
-      forward. (* tgt->t=p; *)  
-      forward. (* p->key=x; *)
-      forward. (* p->value=value; *)
-      forward. (* p->left=NULL; *)
-      forward. (* p->right=NULL; *)
-      assert_PROP (t1= (@E _)) by entailer!.
-      subst t1. simpl node_rep.
-      assert_PROP (field_compatible t_struct_tree_t [] p1) by entailer!.
-      forward_call(lock1, lsh2, t_lock_pred_base p1 lock1, t_lock_pred p1 lock1).
-      { lock_props.
-        setoid_rewrite t_lock_pred_def at 4.
-        Exists (T E x v E) p'. cancel. simpl. Exists p1' p2' l1 l2. unfold ltree. entailer!.
-        rewrite <- later_sepcon; eapply derives_trans; [|apply sepcon_derives, derives_refl; apply now_later].
-        entailer!.
-        { rewrite field_compatible_cons in H6, H8; destruct H6, H8; auto. } }
-      forward. (* return; *)
-    + (* else clause *)
-      destruct t1.
-      { simpl node_rep. normalize. }
-      simpl node_rep.
-      Intros pa pb locka lockb.
-      forward. (* y=p->key; *)
-      forward_if; [ | forward_if ].
-      - (* Inner if, then clause: x<k *)
-        forward.
-        forward.
-        unfold_data_at (data_at _ _ _ tp).
-        rewrite (field_at_data_at _ _ [StructField _left]); simpl.
-        assert_PROP (field_compatible t_struct_tree [StructField _left] tp) by entailer!.
-        rewrite field_compatible_field_address by auto.
-        unfold ltree at 1; Intros.
-        forward.
-        forward_call (locka, lsh1, t_lock_pred pa locka).
-        rewrite t_lock_pred_def at 2.
-        Intros ta tpa.
-        forward_call(lock1, lsh2, t_lock_pred_base p1 lock1, t_lock_pred p1 lock1).
-        { lock_props.
-          setoid_rewrite t_lock_pred_def at 4. Exists (T t1_1 k v0 t1_2) tp.
-          cancel. simpl. Exists pa pb locka lockb.
-          unfold ltree; entailer!.
-          unfold_data_at (data_at _ _ _ tp); cancel.
-          rewrite (field_at_data_at _ _ [StructField _left]), field_compatible_field_address by auto; simpl; cancel.
-          rewrite <- later_sepcon; eapply derives_trans; [|apply sepcon_derives, derives_refl; apply now_later].
-          cancel. }
-        Exists pa locka.
-        unfold ltree; entailer!.
-        unfold t_lock_pred_base.
-        Exists ta tpa; cancel.
-      - (* Inner if, second branch:  k<x *)
-        forward.
-        forward.
-        unfold_data_at (data_at _ _ _ tp).
-        rewrite (field_at_data_at _ _ [StructField _left]); simpl.
-        assert_PROP (field_compatible t_struct_tree [StructField _left] tp) by entailer!.
-        rewrite field_compatible_field_address by auto.
-        unfold ltree at 2; Intros.
-        forward.
-        forward_call (lockb, lsh1, t_lock_pred pb lockb).
-        rewrite t_lock_pred_def at 2.
-        Intros tb tpb.
-        forward_call(lock1, lsh2, t_lock_pred_base p1 lock1, t_lock_pred p1 lock1).
-        { lock_props.
-          setoid_rewrite t_lock_pred_def at 4. Exists (T t1_1 k v0 t1_2) tp.
-          cancel. simpl. Exists pa pb locka lockb.
-          unfold ltree; entailer!.
-          unfold_data_at (data_at _ _ _ tp); cancel.
-          rewrite (field_at_data_at _ _ [StructField _left]), field_compatible_field_address by auto; simpl; cancel.
-          rewrite <- later_sepcon; eapply derives_trans; [|apply sepcon_derives, derives_refl; apply now_later].
-          cancel. }
-        Exists pb lockb.
-        unfold ltree; entailer!.
-        unfold t_lock_pred_base.
-        Exists tb tpb; cancel.
-      - (* x = k *)
-        forward.
-        forward_call(lock1, lsh2, t_lock_pred_base p1 lock1, t_lock_pred p1 lock1).
-        { lock_props.
-          setoid_rewrite t_lock_pred_def at 2. Exists (T t1_1 k v t1_2) tp.
-          cancel. simpl. Exists pa pb locka lockb.
-          unfold ltree; entailer!.
-          rewrite <- later_sepcon; eapply derives_trans; [|apply sepcon_derives, derives_refl; apply now_later].
-          cancel. }
-        forward.
-  * (* After the loop *)
-    forward.
-    unfold loop2_ret_assert. apply andp_left2. normalize.
-Qed.
 
 
